{
 "cells": [
  {
   "cell_type": "code",
   "execution_count": null,
   "id": "934feaba-a7eb-4397-979a-85cc0383681b",
   "metadata": {},
   "outputs": [],
   "source": [
    "#7$ Find the val%e of T(2) for the rec%rrence relation T(n) = 3T(n-1) + 12n, given that T(0)=5.\n",
    "\n",
    "1.Recurrence Relation is T(n) = 3T(n-1) + 12n,\n",
    "\n",
    "So if n=1,T(1)=3*5+12*1 =27 ,T(0)=5 is given in question\n",
    "\n",
    "2.Recurrence Relation is T(n) = 3T(n-1) + 12n,\n",
    "\n",
    "So if n=2,T(2)=3*27+12*2=105  \n",
    "\n",
    "\n",
    "\n"
   ]
  },
  {
   "cell_type": "code",
   "execution_count": null,
   "id": "f7426867-d214-4cae-987e-932d3dfd382c",
   "metadata": {},
   "outputs": [
    {
     "ename": "SyntaxError",
     "evalue": "unterminated string literal (detected at line 9) (4115914174.py, line 9)",
     "output_type": "error",
     "traceback": [
      "\u001b[0;36m  Cell \u001b[0;32mIn[1], line 9\u001b[0;36m\u001b[0m\n\u001b[0;31m    Let's say that your base case is T(1) = b,\u001b[0m\n\u001b[0m       ^\u001b[0m\n\u001b[0;31mSyntaxError\u001b[0m\u001b[0;31m:\u001b[0m unterminated string literal (detected at line 9)\n"
     ]
    }
   ],
   "source": [
    "#2.Given a rec%rrence relation, solve it %sing the s%bstit%tion method:\n",
    "#a. T(n) = T(n-1) + c\n",
    "#b. T(n) = 2T(n/2) + n\n",
    "#c. T(n) = 2T(n/2) + c\n",
    "#d. T(n) = T(n/2) + c\n",
    "\n",
    "(a)\n",
    "\n",
    "Let's say that your base case is T(1) = b, \n",
    "\n",
    "T(2) = T(1) + c = b + c\n",
    "\n",
    "T(3) = T(2) + c = b + c + c\n",
    "\n",
    "\n",
    "\n",
    "T(4) = T(3) + c = b + c + c + c\n",
    "\n",
    "T(5) = T(4) + c = b + c + c + c + c\n",
    "\n",
    "So now the pattern becomes clear:\n",
    "\n",
    "T(n) = b + (n-1)c for n >= 2, and the base case of T(1) = b\n",
    "\n",
    "\n",
    "(b)\n",
    "\n",
    "\n",
    "T(n)=2T(n/2) + n\n",
    "\n",
    "\n",
    "\n",
    "T(n/2)=2T(n/4)+n/2\n",
    "\n",
    "T(N/4)=2T(n/8)+n/4\n",
    "\n",
    "T(n/2)=2T(n/4)+n/2\n",
    "\n",
    "      =2[T(n/4)+n/2]+n\n",
    "      =2**3T(n/2**3)+ 3n\n",
    "      =\n",
    "\n",
    "Next will be : =2**4T(n/2**4)+ 4n\n",
    "\n",
    "Generalise: 2**kT(n/2**k)+ kn\n",
    "\n",
    "Sunstitute n/(2**k)=1\n",
    "\n",
    "n+nlogn\n",
    "\n",
    "\n",
    "c. T(n) = 2T(n/2) + c\n",
    "\n",
    "T(n)=2T(n/2)+c\n",
    "     =2{2T(n/4)+c)+c\n",
    "     =4T(n/4)+3c\n",
    "     =n.T(1)+(n-1)c\n",
    "     =n.c+(n-1)c\n",
    "     =2nc-c\n",
    "     =O(n).\n"
   ]
  },
  {
   "cell_type": "code",
   "execution_count": null,
   "id": "ef900605-c36f-4591-939e-d9c59f974f8d",
   "metadata": {},
   "outputs": [],
   "source": [
    "#3 Recursive Tree approach\n",
    "\n",
    "(a)T(n) = 2T(n-1) +1\n",
    "\n",
    "Link for Tree :  https://i.stack.imgur.com/APf8B.png\n",
    "\n",
    "Work per Level= 2^n\n",
    "\n",
    "T(n)== θ(2^n)\n",
    "\n",
    "\n",
    "b. T(n) = 2T(n/2) + n\n",
    "\n",
    "In this problem, one can observe that the problem is getting split into two problems of half the initial size. Further the additional cost here equals the size. Hence, after the first division, the recursion tree will have two child nodes with input size n/2. We then proceed in this manner until the final input size becomes 1. Therefore, the final recursion tree will look as follows (note that each node contains only the extra cost that is taken) :\n",
    "    \n",
    "   \n",
    "For Tree Pl refer -  https://iq.opengenus.org/content/images/2022/01/recursex1.png\n",
    "\n",
    "As the recursion tree is complete, it remains to calculate the total sum of the entries. For that, we first need to determine the number of levels in the recursion tree. Since each level of the tree splits each of the nodes in that level to half the size of their parents, one can conclude that the total number of levels here is log2n.\n",
    "\n",
    "The next thing we note here is that in each level, the sum of the nodes is n. Therefore, the overall time complexity is given by:\n",
    "\n",
    "T(n) = n + n + .... log2n times\n",
    "= n ( 1 + 1 + ....log2n times)\n",
    "= n log2n\n",
    "= θ(n log2n)\n",
    "\n",
    "\n",
    "\n",
    "\n"
   ]
  }
 ],
 "metadata": {
  "kernelspec": {
   "display_name": "Python 3 (ipykernel)",
   "language": "python",
   "name": "python3"
  },
  "language_info": {
   "codemirror_mode": {
    "name": "ipython",
    "version": 3
   },
   "file_extension": ".py",
   "mimetype": "text/x-python",
   "name": "python",
   "nbconvert_exporter": "python",
   "pygments_lexer": "ipython3",
   "version": "3.10.8"
  }
 },
 "nbformat": 4,
 "nbformat_minor": 5
}
